Capless/Weakening/Basic.lean
@@ -5,6 +5,23 @@ def VarMap.weaken {Γ : Context n m k} :
   VarMap Γ FinFun.weaken (Γ.var T) := by
   constructor <;> (intros; constructor; trivial)
 
+def VarMap.weaken_ext {Γ : Context n m k} :
+  VarMap
+    (Γ.var T)
+    FinFun.weaken.ext
+    ((Γ.var P).var T.weaken) := by
+  apply VarMap.ext
+  apply VarMap.weaken
+
+def VarMap.weaken_cext_ext {Γ : Context n m k} :
+  VarMap
+    ((Γ.cvar CBinding.bound).var T)
+    FinFun.weaken.ext
+    (((Γ.var P).cvar CBinding.bound).var T.weaken) := by
+  apply VarMap.ext
+  apply VarMap.cext
+  apply VarMap.weaken
+
 def CVarMap.weaken {Γ : Context n m k} :
   CVarMap Γ FinFun.weaken (Γ.cvar b) := by
   constructor <;> (intros; constructor; trivial)
