Capless/Weakening/TypedCont/Term.lean
@@ -1,5 +1,19 @@
 import Capless.Store
+import Capless.Weakening.Typing
 namespace Capless
+
+theorem EType.weaken1_weaken (E : EType n m k) :
+  E.weaken.weaken1 = E.weaken.weaken := by
+  simp [EType.weaken, EType.weaken1, EType.rename_rename]
+  rw [<- FinFun.comp_weaken]
+
+theorem EType.weaken_ex (T : CType n m (k+1)) :
+  (EType.ex T).weaken = EType.ex T.weaken := by
+  simp [EType.weaken, EType.rename, CType.weaken]
+
+theorem EType.weaken_cweaken (E : EType n m k) :
+  E.cweaken.weaken = E.weaken.cweaken := by
+  simp [EType.weaken, EType.cweaken, EType.crename_rename_comm]
 
 theorem TypedCont.weaken
   (h : TypedCont Γ E t E') :
@@ -16,8 +30,18 @@ theorem TypedCont.weaken
     rw [heq]
     apply cons
     { rename_i ht _
-      sorry }
+      have ht1 := ht.weaken_ext (P := T)
+      rw [EType.weaken1_weaken] at ht1
+      exact ht1 }
     { exact ih }
-  case conse ih => sorry
+  case conse ih =>
+    simp [Cont.weaken, EType.weaken_ex]
+    apply conse
+    { rename_i ht _
+      have ht1 := ht.weaken_cext_ext (P := T)
+      rw [EType.weaken1_weaken] at ht1
+      rw [EType.weaken_cweaken] at ht1
+      exact ht1 }
+    { exact ih }
 
 end Capless
